prove memory safety for mgf and unify style for types

code/experimental/rsa/Addition.fst
@@ -3,16 +3,10 @@ module Addition
 open FStar.HyperStack.All
 open FStar.Buffer
 open FStar.Int.Cast
+open Lib
 
-module ST = FStar.HyperStack.ST
 module U32 = FStar.UInt32
 module U64 = FStar.UInt64
-
-type bignum = buffer FStar.UInt64.t
-type lbignum (len:U32.t) = 
-     b:bignum{length b = U32.v len} 
-
-type bnlen = (l:U32.t{U32.v l > 0 /\ U32.v l <= 8192})
 
 val sub_loop:
     aLen:bnlen -> bLen:bnlen ->
