code/experimental/rsa/Convert.fst
@@ -4,117 +4,116 @@ open FStar.HyperStack.All
 open FStar.Buffer
 open FStar.Int.Cast
 open Hacl.Endianness
+open Lib
 
 module U32 = FStar.UInt32
 module U8 = FStar.UInt8
 module U64 = FStar.UInt64
 
-type uint8_p = buffer FStar.UInt8.t
-type bignum = buffer FStar.UInt64.t
-
 (* text_to_bn *)
-val get_size_nat: lenText:U32.t{U32.v lenText > 0} -> Tot (res:U32.t{U32.v res > 0})
+val get_size_nat: lenText:U32.t{U32.v lenText > 0} -> Tot (res:bnlen)
 let get_size_nat lenText =
-    U32.(((lenText -^ 1ul) >>^ 3ul) +^ 1ul)
+    let l = U32.(((lenText -^ 1ul) >>^ 3ul) +^ 1ul) in
+    (**) assume(U32.v l > 0 /\ U32.v l <= 8192);
+    l
 
-val bits_to_bn: bits:U32.t{U32.v bits > 0} -> Tot (res:U32.t{U32.v res > 0})
+val bits_to_bn: bits:U32.t{U32.v bits > 0} -> Tot (res:bnlen)
 let bits_to_bn bits =
-    U32.(((bits -^ 1ul) >>^ 6ul) +^ 1ul)
+    let l = U32.(((bits -^ 1ul) >>^ 6ul) +^ 1ul) in
+    (**) assume(U32.v l > 0 /\ U32.v l <= 8192);
+    l
 
-val bits_to_text: bits:U32.t{U32.v bits > 0} -> Tot (res:U32.t{U32.v res > 0})
+val bits_to_text: bits:U32.t{U32.v bits > 0} -> Tot (res:blen)
 let bits_to_text bits =
-    U32.(((bits -^ 1ul) >>^ 3ul) +^ 1ul)
+    let l = U32.(((bits -^ 1ul) >>^ 3ul) +^ 1ul) in
+    (**) assume(U32.v l > 0 /\ U32.v l <= 65536);
+    l
 
 val text_to_nat_loop:
-	input:uint8_p ->
-    res:bignum{disjoint input res} ->
-    len:U32.t{length res = U32.v len /\ FStar.Mul.(8 * U32.v len) < pow2 32 /\ length input = U32.(v (8ul *^ len))} ->
+    len:bnlen ->
+	input:lbytes U32.(8ul *^ len) ->
+    res:lbignum len{disjoint input res} ->
     i:U32.t{U32.v i <= U32.v len} -> Stack unit
     (requires (fun h -> live h input /\ live h res))
     (ensures (fun h0 _ h1 -> live h0 input /\ live h0 res /\
         live h1 input /\ live h1 res /\ modifies_1 res h0 h1))
 
-let rec text_to_nat_loop input res len i =
-    if U32.(i <^ len) then
-        begin
+let rec text_to_nat_loop len input res i =
+    if U32.(i <^ len) then begin
         let inputi = hload64_be (sub input U32.(8ul *^ i) 8ul) in
         let ind = U32.(len -^ i -^ 1ul) in
         res.(ind) <- inputi;
-        text_to_nat_loop input res len U32.(i +^ 1ul)
-        end
-    else ()
+        text_to_nat_loop len input res U32.(i +^ 1ul) end
 
 val text_to_nat:
-    input:uint8_p ->
-    len:U32.t{U32.v len = length input /\ U32.v len > 0} ->
-    res:bignum{length res = U32.v (get_size_nat len) /\ length res > 0 /\ disjoint input res} -> Stack unit
+    len:blen ->
+    input:lbytes len ->
+    res:lbignum (get_size_nat len){disjoint input res} -> Stack unit
 	(requires (fun h -> live h input /\ live h res))
 	(ensures (fun h0 _ h1 -> live h0 input /\ live h0 res /\
         live h1 input /\ live h1 res /\ modifies_1 res h0 h1))
 
 #set-options "--z3rlimit 50 --max_fuel 2"
 
-let text_to_nat input len res =
+let text_to_nat len input res =
     push_frame();
     let num_words = get_size_nat len in
-    assert(0 < U32.v num_words);
+    (**) assert(0 < U32.v num_words);
     let m = U32.(len %^ 8ul) in
-    assert(0 <= U32.v m /\ U32.v m < 8);
-    assume(FStar.Mul.(8 * U32.v num_words) < pow2 32);
+    (**) assert(0 <= U32.v m /\ U32.v m < 8);
+    (**) assume(FStar.Mul.(8 * U32.v num_words) <= 65536);
     let tmpLen = U32.(8ul *^ num_words) in
-    assert(FStar.Mul.(U32.(8 <= 8 * U32.v num_words)));
-    assert(FStar.Mul.(U32.v tmpLen = 8 * U32.v num_words));
-    assert(8 <= U32.v tmpLen);
-    assert(U32.(8 - (U32.v m) <= 8));
-    assert(U32.(8 - (U32.v m) <= U32.v tmpLen));
+    (**) assert(FStar.Mul.(U32.(8 <= 8 * U32.v num_words)));
+    (**) assert(FStar.Mul.(U32.v tmpLen = 8 * U32.v num_words));
+    (**) assert(8 <= U32.v tmpLen);
+    (**) assert(U32.(8 - (U32.v m) <= 8));
+    (**) assert(U32.(8 - (U32.v m) <= U32.v tmpLen));
     let tmp = create 0uy tmpLen in
     let ind = if U32.(m =^ 0ul) then 0ul else U32.(8ul -^ m) in
     blit input 0ul tmp ind len;
-    text_to_nat_loop tmp res num_words 0ul;
+    text_to_nat_loop num_words tmp res 0ul;
     pop_frame()
 
+
 val nat_to_text_loop:
-	input:bignum ->
-    res:uint8_p{disjoint input res} ->
-    len:U32.t{length input = U32.v len /\ FStar.Mul.(8 * U32.v len) < pow2 32 /\ length res = U32.(v (8ul *^ len))} ->
+    len:bnlen ->
+	input:lbignum len ->
+    res:lbytes U32.(8ul *^ len){disjoint input res} ->
     i:U32.t{U32.v i <= U32.v len} -> Stack unit
     (requires (fun h -> live h input /\ live h res))
     (ensures (fun h0 _ h1 -> live h0 input /\ live h0 res /\
         live h1 input /\ live h1 res /\ modifies_1 res h0 h1))
 
-let rec nat_to_text_loop input res len i =
-    if U32.(i <^ len) then
-        begin
+let rec nat_to_text_loop len input res i =
+    if U32.(i <^ len) then begin
         let ind = U32.(len -^ i -^ 1ul) in
         let tmp = input.(ind) in
         hstore64_be (sub res U32.(8ul *^ i) 8ul) tmp;
-        nat_to_text_loop input res len U32.(i +^ 1ul)
-        end
-    else ()
+        nat_to_text_loop len input res U32.(i +^ 1ul) end
 
 val nat_to_text:
-    input:bignum{length input > 0 } ->
-    len:U32.t{U32.v len > 0 /\ length input = U32.v (get_size_nat len)} ->
-    res:uint8_p{length res = U32.v len /\ disjoint res input} -> Stack unit
+    len:blen ->
+    input:lbignum (get_size_nat len) ->
+    res:lbytes len{disjoint res input} -> Stack unit
 	(requires (fun h -> live h input /\ live h res))
 	(ensures (fun h0 _ h1 -> live h0 input /\ live h0 res /\
         live h1 input  /\ live h1 res /\ modifies_1 res h0 h1))
 
-let nat_to_text input len res =
+let nat_to_text len input res =
     push_frame();
     let num_words = get_size_nat len in
-    assert(0 < U32.v num_words);
+    (**) assert(0 < U32.v num_words);
     let m = U32.(len %^ 8ul) in
-    assert(0 <= U32.v m /\ U32.v m < 8);
-    assume(FStar.Mul.(8 * U32.v num_words) < pow2 32);
+    (**) assert(0 <= U32.v m /\ U32.v m < 8);
+    (**) assume(FStar.Mul.(8 * U32.v num_words) <= 65536);
     let tmpLen = U32.(8ul *^ num_words) in
-    assert(FStar.Mul.(U32.(8 <= 8 * U32.v num_words)));
-    assert(FStar.Mul.(U32.v tmpLen = 8 * U32.v num_words));
-    assert(8 <= U32.v tmpLen);
-    assert(U32.(8 - (U32.v m) <= 8));
-    assert(U32.(8 - (U32.v m) <= U32.v tmpLen));
+    (**) assert(FStar.Mul.(U32.(8 <= 8 * U32.v num_words)));
+    (**) assert(FStar.Mul.(U32.v tmpLen = 8 * U32.v num_words));
+    (**) assert(8 <= U32.v tmpLen);
+    (**) assert(U32.(8 - (U32.v m) <= 8));
+    (**) assert(U32.(8 - (U32.v m) <= U32.v tmpLen));
     let tmp = create 0uy tmpLen in
-    nat_to_text_loop input tmp num_words 0ul;
+    nat_to_text_loop num_words input tmp 0ul;
     let ind = if U32.(m =^ 0ul) then 0ul else U32.(8ul -^ m) in
     blit tmp ind res 0ul len;
     pop_frame()
