code/experimental/rsa/MGF.fst
@@ -7,20 +7,13 @@ open FStar.All
 open FStar.Mul
 
 open Convert
+open Lib
 
 module U32 = FStar.UInt32
 module U8 = FStar.UInt8
 
-type uint8_p = buffer FStar.UInt8.t
-type lbytes (len:U32.t) =
-     b:uint8_p{length b = U32.v len}
-
-type blen = (l:U32.t{U32.v l > 0 /\ U32.v l <= 8192})
-
-inline_for_extraction let hLen = 32ul
-
 val hash_sha256:
-	mHash:lbytes hLen ->
+	mHash:lbytes 32ul ->
 	len:blen ->
 	m:lbytes len{disjoint mHash m} -> Stack unit
 	(requires (fun h -> live h m /\ live h mHash))
@@ -28,14 +21,14 @@ val hash_sha256:
 	 	live h1 m /\ live h1 mHash /\ modifies_1 mHash h0 h1))
 let hash_sha256 mHash len m = SHA2_256.hash mHash m len
 
-type mgf_state (mgfseedLen:blen) (accLen:blen) = lbytes U32.((mgfseedLen +^ 4ul) +^ 4ul +^ 32ul +^ accLen)
+type mgf_state (accLen:blen) = lbytes U32.(32ul +^ 4ul +^ 4ul +^ 32ul +^ accLen)
 
-let get_mgfseed_counter #m #a (st:mgf_state m a) : lbytes U32.(m +^ 4ul) = Buffer.sub st 0ul U32.(m +^ 4ul)
-let get_counter #m #a (st:mgf_state m a) : lbytes 4ul = Buffer.sub st U32.(m +^ 4ul) 4ul 
-let get_mHash #m #a (st:mgf_state m a) : lbytes 32ul = Buffer.sub st U32.(m +^ 4ul +^ 4ul) 32ul
-let get_acc #m #a (st:mgf_state m a) : lbytes a = Buffer.sub st U32.(m +^ 4ul +^ 4ul +^ 32ul) a
+let get_mgfseed_counter #a (st:mgf_state a) : lbytes U32.(32ul +^ 4ul) = Buffer.sub st 0ul U32.(32ul +^ 4ul)
+let get_counter #a (st:mgf_state a) : lbytes 4ul = Buffer.sub st U32.(32ul +^ 4ul) 4ul 
+let get_mHash #a (st:mgf_state a) : lbytes 32ul = Buffer.sub st U32.(32ul +^ 4ul +^ 4ul) 32ul
+let get_acc #a (st:mgf_state a) : lbytes a = Buffer.sub st U32.(32ul +^ 4ul +^ 4ul +^ 32ul) a
 
-let mgf_state_inv m a (st:mgf_state m a) = 
+let mgf_state_inv a (st:mgf_state a) = 
            let mgfseed_counter = get_mgfseed_counter st in
 		   let counter = get_counter st in
            let mHash = get_mHash st in
@@ -51,57 +44,66 @@ let mgf_state_inv m a (st:mgf_state m a) =
 		 disjoint counter acc /\
 	     disjoint mHash acc
 
-let mgf_state_st_inv (mLen:blen) (aLen:blen) (st:mgf_state mLen aLen) (h:FStar.HyperStack.mem) = 
-	     mgf_state_inv mLen aLen st /\ live h st
+let mgf_state_st_inv (aLen:blen) (st:mgf_state aLen) (h:FStar.HyperStack.mem) = 
+	     mgf_state_inv aLen st /\ live h st
 
 val mgf_loop:
-	mgfseedLen:blen -> mgfseed:lbytes mgfseedLen ->
-	accLen:blen -> st:mgf_state mgfseedLen accLen {disjoint st mgfseed} ->
-	counter:U32.t{32 * (U32.v counter + 1) <= U32.v accLen} -> Stack unit
-	(requires (fun h -> live h mgfseed /\ mgf_state_st_inv mgfseedLen accLen st h ))
-	(ensures (fun h0 _ h1 -> live h1 mgfseed /\ mgf_state_st_inv mgfseedLen accLen st h1 /\
-			 modifies_1 st h0 h1))
+	count_max:U32.t ->
+	mgfseed:lbytes 32ul ->
+	accLen:blen{U32.v accLen = 32 * (U32.v count_max)} -> 
+	st:mgf_state accLen{disjoint st mgfseed} ->
+	counter:U32.t{U32.v counter <= U32.v count_max} -> Stack unit
+	(requires (fun h -> live h mgfseed /\ mgf_state_st_inv accLen st h ))
+	(ensures (fun h0 _ h1 -> live h0 mgfseed /\ mgf_state_st_inv accLen st h0 /\
+			live h1 mgfseed /\ mgf_state_st_inv accLen st h1 /\
+			modifies_1 st h0 h1))
 
 #set-options "--z3rlimit 150 --max_fuel 2"
 
-let rec mgf_loop mgfseedLen mgfseed accLen st counter =
-	if U32.(32ul *^ counter <^ accLen) then begin
+let rec mgf_loop count_max mgfseed accLen st counter =
+	if U32.(counter <^ count_max) then begin
 		let mgfseed_counter = get_mgfseed_counter st in
 		let c = get_counter st in
 		let mHash = get_mHash st in
 		let acc = get_acc st in
 		
+		(**) assert(length c = 4);
+		(**) assert(length mgfseed_counter = 32 + 4);
 		c.(0ul) <- uint32_to_uint8 (U32.(counter >>^ 24ul));
 		c.(1ul) <- uint32_to_uint8 (U32.(counter >>^ 16ul));
 		c.(2ul) <- uint32_to_uint8 (U32.(counter >>^ 8ul));
 		c.(3ul) <- uint32_to_uint8 counter;
 		
-		(* blit mgfseed 0ul tmp 0ul mgfseedLen; *)
-		blit c 0ul mgfseed_counter mgfseedLen 4ul;
-		(* fill mHash 0uL hLen; *)
-		assume(U32.v mgfseedLen + 4 > 0 /\ U32.v mgfseedLen + 4 <= 8192);
-		hash_sha256 mHash U32.(mgfseedLen +^ 4ul) mgfseed_counter;
+		(* blit mgfseed 0ul tmp 0ul 32ul; *)
+		blit c 0ul mgfseed_counter 32ul 4ul;
+		hash_sha256 mHash U32.(32ul +^ 4ul) mgfseed_counter;
+		(**) assert(length mHash = 32);
+		(**) assert(32 * (U32.v counter) < length acc);
 		blit mHash 0ul acc U32.(32ul *^ counter) 32ul;
-		assert(32 * (U32.v counter + 1) <= U32.v accLen);
-		mgf_loop mgfseedLen mgfseed accLen st U32.(counter +^ 1ul) end
+		mgf_loop count_max mgfseed accLen st U32.(counter +^ 1ul) end
 
-val mgf:
-	mgfseedLen:blen -> mgfseed:lbytes mgfseedLen ->
-	len:blen -> res:lbytes len -> Stack unit
+
+val mgf_sha256:
+	mgfseed:lbytes 32ul ->
+	len:blen -> res:lbytes len{disjoint mgfseed res} -> Stack unit
 	(requires (fun h -> live h res /\ live h mgfseed))
-	(ensures (fun h0 _ h1 -> live h1 res /\ live h1 mgfseed /\ modifies_1 res h0 h1))
+	(ensures (fun h0 _ h1 ->
+		live h0 res /\ live h0 mgfseed /\
+		live h1 res /\ live h1 mgfseed /\ modifies_1 res h0 h1))
 	
-let mgf mgfseedLen mgfseed len res =
-	(* if len > op_Multiply (pow2 32) hLen then failwith "mask too long" *)
+#set-options "--z3rlimit 50"
+
+let mgf_sha256 mgfseed len res =
 	push_frame();
-	let count_max = U32.((len -^ 1ul) /^ hLen +^ 1ul) in
-	let accLen = U32.(hLen *^ count_max) in
-	assume(U32.v accLen > 0 /\ U32.v accLen <= 8192);
-	let accLen: blen = accLen in
-	let st: mgf_state mgfseedLen accLen = create 0uy U32.((mgfseedLen +^ 4ul) +^ 4ul +^ 32ul +^ accLen) in
+	let count_max = U32.((len -^ 1ul) /^ 32ul +^ 1ul) in
+	(**) assume(32 * (U32.v count_max) > 0 /\ 32 * (U32.v count_max) <= 65536);
+	let accLen: blen  = U32.(32ul *^ count_max) in
+	(**) assume(32 + 4 + 4 + 32 + U32.v accLen > 0 /\ 32 + 4 + 4 + 32 + U32.v accLen <= 65536);
+	let stLen = U32.(32ul +^ 4ul +^ 4ul +^ 32ul +^ accLen) in
+	let st: mgf_state accLen = create 0uy stLen in
 	let mgfseed_counter = get_mgfseed_counter st in
-	blit mgfseed 0ul mgfseed_counter 0ul mgfseedLen;
-	mgf_loop mgfseedLen mgfseed accLen st 0ul;
+	blit mgfseed 0ul mgfseed_counter 0ul 32ul;
+	mgf_loop count_max mgfseed accLen st 0ul;
 	let acc = get_acc st in
 	blit acc 0ul res 0ul len;
 	pop_frame()
