code/experimental/rsa/Comparison.fst
@@ -3,37 +3,38 @@ module Comparison
 open FStar.HyperStack.All
 open FStar.Buffer
 open FStar.Int.Cast
+open Lib
 
 module U32 = FStar.UInt32
 module U64 = FStar.UInt64
 module I32 = FStar.Int32
 
-type bignum = buffer FStar.UInt64.t
-
 val isMore_loop:
-    a:bignum ->
-    b:bignum{length b = length a} ->
+    aLen:bnlen ->
+    bLen:bnlen{U32.v aLen = U32.v bLen} ->
+    a:lbignum aLen ->
+    b:lbignum bLen{disjoint a b} ->
     count:U32.t{U32.v count <= length a} -> Stack bool
     (requires (fun h -> live h a /\ live h b))
 	(ensures (fun h0 _ h1 -> live h0 a /\ live h0 b
          /\ live h1 a /\ live h1 b /\ h0 == h1))
 
-let rec isMore_loop a b count =
+let rec isMore_loop aLen bLen a b count =
     if U32.(count >^ 0ul) then
         let count = U32.(count -^ 1ul) in
         let t1 = a.(count) in
         let t2 = b.(count) in
         (if not (U64.(t1 =^ t2)) then
             if U64.(t1 >^ t2) then true else false
-        else isMore_loop a b count)
+        else isMore_loop aLen bLen a b count)
     else false
 
 (* if a > b then true else false *)
 val isMore:
-    aLen:U32.t{U32.v aLen > 0} ->
-    bLen:U32.t{U32.v bLen > 0} ->
-    a:bignum{length a = U32.v aLen} ->
-    b:bignum{length b = U32.v bLen /\ disjoint a b} -> Stack bool
+    aLen:bnlen ->
+    bLen:bnlen ->
+    a:lbignum aLen ->
+    b:lbignum bLen{disjoint a b} -> Stack bool
     (requires (fun h -> live h a /\ live h b))
     (ensures (fun h0 _ h1 -> live h0 a /\ live h0 b
         /\ live h1 a /\ live h1 b /\ h0 == h1))
@@ -41,4 +42,4 @@ val isMore:
 let isMore aLen bLen a b =
     if U32.(aLen >^ bLen) then true
     else if U32.(aLen <^ bLen) then false
-         else isMore_loop a b aLen
+         else isMore_loop aLen bLen a b aLen
