code/experimental/rsa/Lib.fst
@@ -1,0 +1,18 @@
+module Lib
+
+open FStar.HyperStack.All
+open FStar.Buffer
+open FStar.Int.Cast
+open FStar.All
+open FStar.Mul
+
+module U32 = FStar.UInt32
+module U64 = FStar.UInt64
+
+type uint8_p = buffer FStar.UInt8.t
+type lbytes (len:U32.t) = b:uint8_p{length b = U32.v len}
+type blen = (l:U32.t{U32.v l > 0 /\ U32.v l <= 65536})
+
+type bignum = buffer FStar.UInt64.t
+type lbignum (len:U32.t) = b:bignum{length b = U32.v len}
+type bnlen = (l:U32.t{U32.v l > 0 /\ U32.v l <= 8192})
