code/experimental/rsa/Shift.fst
@@ -3,26 +3,27 @@ module Shift
 open FStar.HyperStack.All
 open FStar.Buffer
 open FStar.Int.Cast
+open Lib
 
 module U32 = FStar.UInt32
 module U64 = FStar.UInt64
 
-type bignum = buffer FStar.UInt64.t
-
 let bn_tbit = 0x8000000000000000uL
 
 val lshift_loop:
-    a:bignum{length a > 0} ->
+    aLen:bnlen ->
+    resLen:bnlen ->
+    a:lbignum aLen ->
     count:U32.t{U32.v count <= length a} ->
     nw:U32.t -> lb:U32.t{0 < U32.v lb /\ U32.v lb < 64} ->
-    res:bignum{length res = length a + U32.v nw + 1 /\ U32.v count + U32.v nw < length res /\ disjoint a res} -> 
+    res:lbignum resLen{U32.v count + U32.v nw < length res /\ disjoint a res} -> 
     Stack unit
 	(requires (fun h -> live h a /\ live h res))
 	(ensures (fun h0 _ h1 -> live h0 a /\ live h0 res /\ 
         live h1 a /\ live h1 res /\ modifies_1 res h0 h1))
 
-let rec lshift_loop a count nw lb res =
-    if U32.(count >^ 0ul) then
+let rec lshift_loop aLen resLen a count nw lb res =
+    if U32.(count >^ 0ul) then begin
         let ind = U32.(nw +^ count) in
         let tmp = res.(ind) in
         let count = U32.(count -^ 1ul) in
@@ -31,55 +32,53 @@ let rec lshift_loop a count nw lb res =
         assert(0 < U32.v rb /\ U32.v rb < 64);
         res.(ind) <- U64.(tmp |^ U64.(t1 >>^ rb));
         res.(U32.(ind -^ 1ul)) <- U64.(t1 <<^ lb);
-        lshift_loop a count nw lb res
-    else ()
+        lshift_loop aLen resLen a count nw lb res end
 
 (* res = a << n *)
 val lshift:
-    aLen:U32.t{U32.v aLen > 0} ->
-    a:bignum{length a = U32.v aLen} -> 
-    nCount:U32.t ->
-    res:bignum{length res = U32.v aLen + U32.v nCount / 64 + 1 /\ disjoint a res} -> 
+    aLen:bnlen ->
+    a:lbignum aLen ->
+    nCount:U32.t{U32.v nCount > 0} ->
+    res:lbignum U32.(aLen +^ nCount /^ 64ul +^ 1ul){disjoint a res} ->
     Stack unit
 	(requires (fun h -> live h a /\ live h res))
-	(ensures (fun h0 _ h1 -> live h0 a /\ live h0 res /\ 
+	(ensures (fun h0 _ h1 -> live h0 a /\ live h0 res /\
         live h1 a /\ live h1 res /\ modifies_1 res h0 h1))
 
 let lshift aLen a nCount res =
     let nw = U32.(nCount/^ 64ul) in
     let resLen = U32.(aLen +^ nw +^ 1ul) in
+    (**) assume(U32.v resLen > 0 /\ U32.v resLen <= 8192);
     let lb = U32.(nCount %^ 64ul) in
     (if U32.(lb =^ 0ul) then
         blit a 0ul res nw aLen
-    else lshift_loop a aLen nw lb res)
-
+    else lshift_loop aLen resLen a aLen nw lb res)
 
 val rshift1_loop:
-    a:bignum -> 
-    carry:U64.t -> 
+    aLen:bnlen ->
+    a:lbignum aLen ->
+    carry:U64.t ->
     ind:U32.t{U32.v ind < length a} ->
-    res:bignum{U32.v ind < length res /\ length res = length a} -> 
-    Stack unit
+    res:lbignum aLen{disjoint a res} -> Stack unit
     (requires (fun h -> live h a /\ live h res))
 	(ensures (fun h0 _ h1 -> live h0 a /\ live h0 res /\ 
         live h1 a /\ live h1 res /\ modifies_1 res h0 h1))
 
-let rec rshift1_loop a carry ind res =
-    if U32.(ind >^ 0ul) then
+let rec rshift1_loop aLen a carry ind res =
+    if U32.(ind >^ 0ul) then begin
         let ind = U32.(ind -^ 1ul) in
         let tmp = a.(ind) in
         res.(ind) <- U64.((tmp >>^ 1ul) |^ carry);
         let carry = if U64.((tmp &^ 1uL) =^ 1uL) then bn_tbit else 0uL in
-        rshift1_loop a carry ind res
-    else ()
+        rshift1_loop aLen a carry ind res end
 
 (* res = a >> 1 *)
 val rshift1:
-    aLen:U32.t{U32.v aLen > 0} ->
-    a:bignum{length a = U32.v aLen} ->
-    res:bignum{length res = U32.v aLen} -> Stack unit
+    aLen:bnlen ->
+    a:lbignum aLen ->
+    res:lbignum aLen{disjoint a res} -> Stack unit
 	(requires (fun h -> live h a /\ live h res))
-	(ensures (fun h0 _ h1 -> live h0 a /\ live h0 res /\ 
+	(ensures (fun h0 _ h1 -> live h0 a /\ live h0 res /\
         live h1 a /\ live h1 res /\ modifies_1 res h0 h1))
 
 #set-options "--z3rlimit 50"
@@ -90,4 +89,4 @@ let rshift1 aLen a res =
     let carry = if U64.((tmp &^ 1uL) =^ 1uL) then bn_tbit else 0uL in
     let tmp = U64.(tmp >>^ 1ul) in
     (if U64.(tmp >^ 0uL) then res.(i) <- tmp);
-    rshift1_loop a carry i res
+    rshift1_loop aLen a carry i res
