code/experimental/rsa/Test.RSA.fst
@@ -10,15 +10,16 @@ module U32 = FStar.UInt32
 type uint8_p = buffer FStar.UInt8.t
 type bignum = buffer FStar.UInt64.t
 
-val ctest:modBits:U32.t -> pkeyBits:U32.t -> skeyBits:U32.t -> msgLen:U32.t ->
+val ctest:
+    modBits:U32.t -> pkeyBits:U32.t -> skeyBits:U32.t -> msgLen:U32.t ->
 	n:uint8_p -> e:uint8_p -> d:uint8_p -> msg:uint8_p -> salt:uint8_p -> Stack bool
 	(requires (fun h -> True))
 	(ensures  (fun h0 r h1 -> True))
 let ctest modBits pkeyBits skeyBits msgLen n e d msg salt =
 	push_frame();
-	let nNat = create 0uL (bits_to_bn modBits) in text_to_nat n (bits_to_text modBits) nNat;
-	let eNat = create 0uL (bits_to_bn pkeyBits) in text_to_nat e (bits_to_text pkeyBits) eNat;
-	let dNat = create 0uL (bits_to_bn skeyBits) in text_to_nat d (bits_to_text skeyBits) dNat;
+	let nNat = create 0uL (bits_to_bn modBits)  in text_to_nat (bits_to_text modBits)  n nNat;
+	let eNat = create 0uL (bits_to_bn pkeyBits) in text_to_nat (bits_to_text pkeyBits) e eNat;
+	let dNat = create 0uL (bits_to_bn skeyBits) in text_to_nat (bits_to_text skeyBits) d dNat;
 	let pkey = Mk_rsa_pubkey nNat eNat in
 	let skey = Mk_rsa_privkey pkey dNat in
 	let sgnt = create 0uy (bits_to_text modBits) in
@@ -234,6 +235,6 @@ val main: unit -> Stack FStar.Int32.t
 	(requires (fun h -> True))
 	(ensures  (fun h0 r h1 -> True))
 let main () =
-	let test = test1() && test2() && test3() && test4()  in
+	let test = test1() && test2() && test3() && test4() in
     if test then C.print_string (C.string_of_literal "SUCCESS") else C.print_string (C.string_of_literal "Test failed");
     C.exit_success
